theories/iris/examples/stack_robust.v
@@ -18,6 +18,8 @@ Close Scope byte_scope.
 Section Client.
   Context `{!wasmG Σ, !hvisG Σ, !hmsG Σ}.
 
+  Definition xx i := (VAL_int32 (Wasm_int.int_of_Z i32m i)).
+  
   Definition main :=
     [ BI_call 0 ;
       BI_tee_local 0 ;
@@ -278,16 +280,16 @@ Section Client_main.
          ∗ (∃ gv, N.of_nat k ↦[wg] {| g_mut := MUT_mut; g_val := gv |})
          (* new stack *)
          ∗ N.of_nat idf0 ↦[wf]FC_func_native istack (Tf [] [T_i32]) l0 f0
-         ∗ spec0_new_stack idf0 istack l0 f0 isStack newStackAddrIs
+         ∗ spec0_new_stack idf0 istack l0 f0 isStack newStackAddrIs ⊤
          (* push *)
          ∗ N.of_nat idf4↦[wf]FC_func_native istack (Tf [T_i32; T_i32] []) l4 f4
-         ∗ spec4_push idf4 istack l4 f4 isStack
+         ∗ spec4_push idf4 istack l4 f4 isStack ⊤
          (* pop *)
          ∗ N.of_nat idf3↦[wf]FC_func_native istack (Tf [T_i32] [T_i32]) l3 f3
-         ∗ spec3_pop idf3 istack l3 f3 isStack
+         ∗ spec3_pop idf3 istack l3 f3 isStack ⊤
          (* map *)
          ∗ N.of_nat idf5↦[wf]FC_func_native istack (Tf [T_i32; T_i32] []) l5 f5
-         ∗ spec5_stack_map_trap idf5 istack l5 f5 isStack idt 
+         ∗ spec5_stack_map_trap idf5 istack l5 f5 isStack idt ⊤
          (* table *)
          ∗ N.of_nat idt↦[wtblock]table_init_replace_single stacktab (nat_of_int (Wasm_int.Int32.repr 0)) [Some a]
          (* new stack predicate *)
@@ -368,7 +370,7 @@ Section Client_main.
       iApply wp_value;[unfold IntoVal;by eapply of_to_val|].
       iIntros (LI HLI%lfilled_Ind_Equivalent);inversion HLI;subst. iSimpl.
       inversion H8;subst. iSimpl.
-      match goal with |- context [ WP ?e {{ _ }}%I ] => set (v:=e) end.
+      match goal with |- context [ WP ?e @ _ {{ _ }}%I ] => set (v:=e) end.
       eassert (iris.to_val v = Some (retV (SH_rec _ _ _ (SH_base [] []) _))) as Hval'.
       { cbn. eauto. }
       iApply wp_value;[unfold IntoVal;by eapply of_to_val|].
@@ -652,14 +654,15 @@ Section Client_instantiation.
           na_own logrel_nais ⊤ ∗
           (∃ name, 8%N ↪[vis] {| modexp_name := name; modexp_desc := MED_global (Mk_globalidx (N.to_nat g_ret)) |}) ∗
           (∃ vs0 vs1 vs2 vs3 vs4 vs5 vs6, [∗ list] v↦vs∈[vs0;vs1;vs2;vs3;vs4;vs5;vs6], N.of_nat v ↪[vis] vs) ∗
-          (∃ vs, 7%N ↪[vis] vs)
+          (∃ vs, 7%N ↪[vis] vs) ∗
+          ↪[frame] empty_frame
       }}}
         ((stack_adv_client_instantiate,[]) : host_expr)
       {{{ v, ⌜v = (trapHV : host_val)⌝ ∨ ∃ v, g_ret ↦[wg] {| g_mut := MUT_mut; g_val := VAL_int32 v|} }}} .
   Proof.
     iIntros (Htyp Hnostart Hrestrict Hboundst Hboundsm Hgrettyp).
     iModIntro. iIntros (Φ) "(Hgret & Hmod_stack & Hmod_adv & Hmod_lse & Hown & Hvis8 & 
-                        Hvisvst & Hvis7) HΦ".
+                        Hvisvst & Hvis7 & Hemptyframe) HΦ".
     iDestruct "Hvisvst" as (vs0 vs1 vs2 vs3 vs4 vs5 vs6) "Hvis".
     iApply (wp_seq_host_nostart with "[$Hmod_stack] [Hvis] ") => //.
     { iIntros "Hmod_stack".
@@ -791,21 +794,6 @@ Section Client_instantiation.
     iDestruct (mapsto_frac_ne with "Hadvf Himpfcl3") as "%Hadv3" ; first by eauto.
     iDestruct (mapsto_frac_ne with "Hadvf Himpfcl4") as "%Hadv4" ; first by eauto.
     iDestruct (mapsto_frac_ne with "Hadvf Himpfcl5") as "%Hadv5" ; first by eauto.
- (*   repeat (apply Forall2_cons in Hft; destruct Hft as [Heq Hft];
-    simpl in Heq; destruct Heq as [cl [Heqcl _]];
-    repeat (rewrite lookup_insert in Heqcl + (rewrite lookup_insert_ne in Heqcl;[|done])); 
-    inversion Heqcl; subst cl; clear Heqcl).
-    
-    (apply Forall2_cons in Hft; destruct Hft as [Heq Hft];
-    simpl in Heq; destruct Heq as [cl [Heqcl _]];
-    repeat (rewrite lookup_insert in Heqcl + (rewrite lookup_insert_ne in Heqcl;[|done])); 
-    inversion Heqcl). subst cl; clear Heqcl).
-    apply Forall2_cons in Hft; destruct Hft as [Heq Hft];
-    simpl in Heq; destruct Heq as [cl [Heqcl _]]).
-    do 1 rewrite lookup_insert_ne in Heqcl => //. rewrite lookup_insert in Heqcl.
-    inversion Heqcl; subst cl; clear Heqcl.
-    apply all2_Forall2 in Hft.
-    repeat (rewrite lookup_insert + (rewrite lookup_insert_ne;[|done])).*)
     repeat (rewrite lookup_insert + (rewrite lookup_insert_ne;[|done])).
     iDestruct "Hcl0" as %[Heq1 Heq2];inversion Heq1;inversion Heq2;clear Heq1 Heq2.
     iDestruct "Hcl1" as %[Heq1 Heq2];inversion Heq1;inversion Heq2;clear Heq1 Heq2.
@@ -817,11 +805,16 @@ Section Client_instantiation.
     iDestruct "Hidtab" as (tab tt) "[Hidtab [%Heq %Htt]]". inversion Heq;subst tab.
 
     iApply (wp_wand_host _ _ _ (λ v, _ ∗ ↪[frame]empty_frame)%I with "[-HΦ] [HΦ]");cycle 1.
-    { iIntros (v) "[Hv ?]". iApply "HΦ". iExact "Hv". }
+    { iIntros (v) "[Hv Hframe]". iApply "HΦ". iExact "Hv". }
 
-    iApply (instantiation_spec_operational_start with "[Hmod_lse HimpsH Himpfcl0 Himpfcl1 Himpfcl2 Himpfcl3 Himpfcl4 
-                                                 Himpfcl5 Hadvf Hidtab Hn Hgret Hvis8]")
+    iApply (instantiation_spec_operational_start with "[$Hemptyframe] [Hmod_lse HimpsH Himpfcl0 Himpfcl1 Himpfcl2 Himpfcl3 Himpfcl4 Himpfcl5 Hadvf Hidtab Hn Hgret Hvis8]")
     ; try exact client_module_typing;[eauto|..].
+    { unfold module_restrictions.
+      simpl.
+      split; first by exists [].
+      split; first by exists ([Wasm_int.int_of_Z i32m 0]).
+      by exists [].
+    }
     { iFrame. 
       instantiate (5:=[_;_;_;_;_;_;_;_;_]).
       iDestruct "HimpsH" as "($&$&$&$&$&$&$&_)". iFrame "Hn Hvis8".
