theories/iris/iris_wasm_determ.v
@@ -2,7 +2,7 @@ From mathcomp Require Import ssreflect eqtype seq ssrbool.
 From iris.program_logic Require Import language.
 From iris.proofmode Require Import tactics.
 From iris.base_logic Require Export gen_heap proph_map.
-Require Export iris iris_locations stdpp_aux.
+Require Export stdpp_aux.
 Require Export datatypes host operations properties opsem.
 Require Import iris_reduce_properties iris_wasm_lang_properties iris_reduction_core iris_split_reduce.
 
